dataplane/Examples/Batch_op.thy
@@ -10,8 +10,8 @@ term "show_list show_nat"
 
 abbreviation "show_myprod \<equiv> (\<lambda> s1 s2. show_prod s1 s2 o to_prod)"
 
-definition batch_op where
-  "batch_op ips ops comb os logic = notifier_op ips ops os 
+definition batch_op_logic where
+  "batch_op_logic ips ops comb os logic = notifier_op ips ops os 
    (\<lambda> os compl_caps.
     let comb_caps = comb compl_caps in
     if (\<forall> p. comb_caps p = []) then trace (STR ''No capabilities'') {||} else
@@ -24,14 +24,14 @@ definition batch_op where
     (drop_caps (produces os (map (\<lambda> (d, cap). (en2 os d, cap)) outs)) drops)) outs_drops)"
 
 
-definition batch_fun_op where
-  "batch_fun_op os f = batch_op {|(1 :: 1)|} {|(1 :: 1)|} id os
+definition batch_op where
+  "batch_op os f = batch_op_logic {|(1 :: 1)|} {|(1 :: 1)|} id os
    (\<lambda> compl_batches ts caps. {| (concat (map (\<lambda> t. map (\<lambda> x. (x, Cap t 1)) (f (compl_batches 1 t))) (ts 1)), map (\<lambda> t. Cap t 1) (caps 1)) |})"
 
 
 (*
 definition diff_op where
-  "diff_op os = batch_op {|(1 :: 2), 2|} {|1|} 
+  "diff_op os = batch_op_logic {|(1 :: 2), 2|} {|1|} 
    (\<lambda> compl_caps p. if p = 1 then filter (\<lambda> t. t \<in> set (compl_caps 2)) (compl_caps 1) else filter (\<lambda> t. t \<in> set (compl_caps 1)) (compl_caps 2))
    (os\<lparr> de1 := projl, en2 := Inr \<rparr>)
    (\<lambda> compl_batches ts caps. 
